SystemFD/Examples/Nat.lean
@@ -7,19 +7,72 @@ import SystemFD.Evaluator
 -- notation t1 ";;" t2 => t1 (t2)
 -- notation t1 "::" t2 => Term.cons t1 t2
 
+namespace Term
+  @[simp]
+  def succ : Term -> Term
+  | .var x => var (x + 1)
+  | t => t
+
+  @[simp]
+  def add : Term -> Nat -> Term
+  | .var x, k => .var (x + k)
+  | t, _ => t
+end Term
+
 def NatCtx : Ctx Term := [
-    .ctor (#1 -t> #1),
-    .ctor #0,
+    -- instance fix = Λ a. λ i. guard (Fix a) <- i then λ f. f (fix i f)
+    .inst 0 (Λ[★] `λ[#3 `@k #0] `λ[#1 -t> #2]
+      .guard (#4 `@t #2) #1
+        (#0 `@ (#3 `@t #2 `@ #1 `@ #0))),
+    -- .inst 0 (Λ[★] `λ[#3 `@k #0]
+    --   .guard (#3 `@t #1) #0
+    --     (`λ[#1 -t> #1] #0 `@ (#2 `@ #1 `@ #0))),
+    -- open fix : ∀ a, Fix a -> (a -> a) -> a
+    .openm (∀[★] #2 `@k #0 -t> (#1 -t> #2) -t> #2),
+    -- instance Fix : ∀ a, Fix a
+    .insttype (∀[★] #1 `@k #0),
+    -- open Fix : ★ -> ◯
+    .opent (★ -k> ◯),
+    -- Nat.succ
+    .ctor (#1 -t> #2),
+    -- Nat.zero
+    .ctor #0, -- Nat.zero
+    -- Nat
     .datatype ★
   ]
 
-def ex_pred : Term := `λ[#2]
-  .ite #2 #0 #0
-  (.ite #1 #0 (`λ[#3] #0) #0)
+  -- #3 : [S' 4](∀[★] #2 `@k #0 -t> (#1 -t> #2) -t> #2)
+  --    : ∀[★] #6 `@k #0 -t> (#1 -t> #2) -t> #2
+  -- #2 : ★
+  -- #1 : [S' 2](#3 `@k #0)
+  --    : #5 `@k #2
+  -- #0 : [S](#1 -t> #2)
+  --    : #2 -t> #3
 
 def ex_succ : Term := #0
 
 
+  -- #3 `@t #2 : (#6 `@k #0 -t> (#1 -t> #2) -t> #2) β[#2]
+  --           : #5 `@k #2 -t> (#3 -t> #4) -t> #4
+
+  -- #3 `@t #2 `@ #1 : ((#3 -t> #4) -t> #4) β[.kind]
+  --                 : (#2 -t> #3) -t> #3
+
+  -- #3 `@t #2 `@ #1 `@ #0 : #3 β[.kind] = #2
+
+def fixi := #0
+def ofixi := fixi.succ
+def Fixi := ofixi.succ
+def oFixi := Fixi.succ
+def succi := oFixi.succ
+def zeroi := succi.succ
+def Nati := zeroi.succ
+
+def ex_pred : Term := `λ[Nati]
+  .ite (zeroi.succ) #0 #0
+  (.ite (succi.succ) #0 (`λ[Nati.succ] #0) #0)
+
+#eval wf_ctx NatCtx
 #eval infer_type NatCtx ex_pred
 #eval infer_type NatCtx ex_succ
 #eval! infer_type NatCtx (ex_pred `@ (ex_succ `@ #1))
