SystemFD/Term/Substitution.lean
@@ -29,7 +29,7 @@ instance instLawfulBEq_SpineVariant : LawfulBEq SpineVariant where
 
 namespace Term
   def to_telescope : Term -> Ctx Term × Term
-  | ctor2 .arrow A B =>
+  | bind2 .arrow A B =>
     let (Γ, r) := to_telescope B
     (.type A::Γ, r)
   | ∀[A] B =>
@@ -58,27 +58,27 @@ namespace Term
   | t, .cons (.type, h) tl => apply_spine (t `@t h) tl
   | t, .cons (.kind, h) tl => apply_spine (t `@k h) tl
 
-  @[simp]
-  def neutral_head : Term -> Option Nat
-  | .var x => .some x
-  | ctor2 .app t _ => neutral_head t
-  | ctor2 .appt t _ => neutral_head t
-  | ctor2 .appk t _ => neutral_head t
-  | _ => .none
+  -- @[simp]
+  -- def neutral_head : Term -> Option Nat
+  -- | .var x => .some x
+  -- | ctor2 .app t _ => neutral_head t
+  -- | ctor2 .appt t _ => neutral_head t
+  -- | ctor2 .appk t _ => neutral_head t
+  -- | _ => .none
 
-  @[simp]
-  def neutral_subst : Term -> Option (Subst Term)
-  | .var _ => .some I
-  | ctor2 .app f a => do
-    let f' <- neutral_subst f
-    .some (.su a :: f')
-  | ctor2 .appt f a => do
-    let f' <- neutral_subst f
-    .some (.su a :: f')
-  | ctor2 .appk f a => do
-    let f' <- neutral_subst f
-    .some (.su a :: f')
-  | _ => .none
+  -- @[simp]
+  -- def neutral_subst : Term -> Option (Subst Term)
+  -- | .var _ => .some I
+  -- | ctor2 .app f a => do
+  --   let f' <- neutral_subst f
+  --   .some (.su a :: f')
+  -- | ctor2 .appt f a => do
+  --   let f' <- neutral_subst f
+  --   .some (.su a :: f')
+  -- | ctor2 .appk f a => do
+  --   let f' <- neutral_subst f
+  --   .some (.su a :: f')
+  -- | _ => .none
 
   @[simp]
   def smap (lf : Subst.Lift Term) (f : Nat -> Subst.Action Term) : Term -> Term
